make Coq proofs closer to paper proofs

partial/Arith.v
@@ -25,17 +25,17 @@ Fixpoint eval (x: Expr) : nat :=
 
 Inductive Code : Set :=
 | LOAD : nat -> Code -> Code
-| ADD : adr -> Code -> Code
-| STORE : adr -> Code -> Code
+| ADD : Reg -> Code -> Code
+| STORE : Reg -> Code -> Code
 | HALT : Code.
 
-Fixpoint comp' (x : Expr) (r : adr) (c : Code) : Code :=
+Fixpoint comp (x : Expr) (r : Reg) (c : Code) : Code :=
   match x with
     Val n => LOAD n c
-  | Add e1 e2 => comp' e1 r (STORE r (comp' e2 (next r) (ADD r c)))
+  | Add e1 e2 => comp e1 r (STORE r (comp e2 (next r) (ADD r c)))
   end.
 
-Definition comp (x : Expr) : Code := comp' x adr0 HALT.
+Definition compile (x : Expr) : Code := comp x first HALT.
 
 (** * Virtual Machine *)
 
@@ -64,7 +64,6 @@ Module VM <: Machine.
 Definition Conf := Conf.
 Definition Pre := cle.
 Definition Rel := VM.
-Definition MemElem := nat.
 Lemma monotone : monotonicity cle VM.
 prove_monotonicity. Qed.
 Lemma preorder : is_preorder cle.
@@ -74,19 +73,14 @@ Module VMCalc := Calculation mem VM.
 Import VMCalc.
 
 
-(** Specification of the compiler *)
+(** Specification of the compiler comp *)
 
-Theorem spec e r c a s : freeFrom r s -> ⟨comp' e r c, a, s⟩  =|> ⟨c , eval e, s⟩ .
+Theorem spec : forall e r c a s, freeFrom r s -> ⟨comp e r c, a, s⟩  =|> ⟨c , eval e, s⟩ .
 
 
 (** Setup the induction proof *)
 
 Proof.
-  intros.
-  generalize dependent c.
-  generalize dependent s.
-  generalize dependent r.
-  generalize dependent a.
   induction e;intros.
 
 (** Calculation of the compiler *)
@@ -112,14 +106,25 @@ Proof.
   <== {apply vm_add}
       ⟨ADD r c, eval e2, s[r:=eval e1]⟩.
   <|= {apply IHe2}
-      ⟨comp' e2 (next r) (ADD r c), eval e1, s[r:=eval e1]⟩.
+      ⟨comp e2 (next r) (ADD r c), eval e1, s[r:=eval e1]⟩.
   <== { apply vm_store}
-    ⟨STORE r (comp' e2 (next r) (ADD r c)), eval e1, s⟩.
+    ⟨STORE r (comp e2 (next r) (ADD r c)), eval e1, s⟩.
   <|= { apply IHe1 }
-    ⟨comp' e1 r (STORE r (comp' e2 (next r) (ADD r c))), a, s⟩.
+    ⟨comp e1 r (STORE r (comp e2 (next r) (ADD r c))), a, s⟩.
   [].
 Qed.
 
+
+(** Specification of the whole compiler *)
+
+Theorem spec' e a : ⟨compile e, a, empty⟩  =|> ⟨HALT , eval e, empty⟩.
+Proof.
+  begin
+    ⟨ HALT, eval e, empty ⟩.
+    <|= {apply spec; apply empty_mem_free}
+    ⟨comp e first HALT, a, empty⟩.
+    [].
+Qed.
 
 (** * Soundness *)
   
@@ -134,10 +139,10 @@ Lemma determ_vm : determ VM.
 Qed.
 
 
-Theorem sound x a s C : freeFrom adr0 s -> ⟨comp x, a, s⟩ =>>! C -> exists s', C = ⟨HALT, eval x, s'⟩.
+Theorem sound x a C : ⟨compile x, a, empty⟩ =>>! C -> exists s, C = ⟨HALT, eval x, s⟩.
 Proof.
-  intros F M.
-  pose (spec x adr0 HALT a s F). unfold Reach in *. repeat autodestruct.
+  intros M.
+  pose (spec' x a). unfold Reach in *. repeat autodestruct.
   pose (determ_trc determ_vm) as D.
   unfold determ in D. inversion H0. subst. eexists. eapply D. apply M. split. 
   apply H. intro Contra. destruct Contra.
