partial/Memory.v
@@ -2,74 +2,84 @@
 
 Create HintDb memory.
 
-
 Module Type Memory.
 
-Parameter adr : Set.
-
-Parameter adr0 : adr.
-Parameter next : adr -> adr.
-
+(* Types *)
+Parameter Reg : Set.
 Parameter Mem : Type -> Type.
 
+(* Operations *)
+Parameter empty : forall {T}, Mem T.
+Parameter set : forall {T}, Reg -> T -> Mem T -> Mem T.
+Parameter get : forall {T}, Reg -> Mem T -> option T.
+Parameter first : Reg.
+Parameter next : Reg -> Reg.
 
-Parameter get : forall {T}, adr -> Mem T -> option T.
-Parameter set : forall {T}, adr -> T -> Mem T -> Mem T.
-
-Parameter freeFrom : forall {T}, adr -> Mem T -> Prop.
+(* Predicates *)
+Parameter freeFrom : forall {T}, Reg -> Mem T -> Prop.
 Parameter memle : forall {T}, Mem T -> Mem T -> Prop.
 
-
+(* Notations *)
 Notation "s ≤ t" := (memle s t) (at level 70) : memory_scope.
 Open Scope memory_scope.
 Notation "s ≥ t" := (t ≤ s) (at level 70) : memory_scope.
-
-
-Axiom get_set : forall T (r : adr) (v : T) (s :  Mem T),
-    get r (set r v s) = Some v.
-
-Axiom set_set : forall T (r : adr) (v v' : T) (s :  Mem T),
-    set r v (set r v' s) = set r v s.
-
-Axiom freeFrom_set : forall {T} r (v : T) s, freeFrom r s ->  freeFrom (next r) (set r v s).
-
-
-Axiom memle_refl : forall {T} (s : Mem T), s ≤ s.
-Axiom memle_trans : forall {T} (s t u : Mem T), s ≤ t -> t ≤ u -> s ≤ u.
-
-
-Axiom memle_set : forall {T} (s : Mem T) r v, freeFrom r s -> s ≤ set r v s.
-Axiom memle_get : forall {T} (s t : Mem T) r v, s ≤ t -> get r s = Some v -> get r t = Some v.
-Axiom set_monotone : forall {T} (s t : Mem T) r v, s ≤ t -> set r v s ≤ set r v t .
-
-
 Notation "s [ r ] = v" := (get r s = Some v) (at level 70).
 Notation "s [ r := v ]" := (set r v s) (at level 70).
 
 
-Hint Resolve memle_set memle_get memle_refl set_monotone memle_trans freeFrom_set : memory.
+(* Property 1 *)
+Axiom empty_mem_free : forall T, freeFrom first (@empty T). 
 
+(* Property 2 *)
+
+Axiom get_set : forall T (r : Reg) (v : T) (s :  Mem T),
+    get r (set r v s) = Some v.
+
+(* Property 3 *)
+
+Axiom memle_set : forall {T} (s : Mem T) r v, freeFrom r s -> s ≤ set r v s.
+
+(* Property 4 *)
+
+Axiom freeFrom_set : forall {T} r (v : T) s, freeFrom r s ->  freeFrom (next r) (set r v s).
+
+(* Property 5 *)
+
+Axiom memle_refl : forall {T} (s : Mem T), s ≤ s.
+Axiom memle_trans : forall {T} (s t u : Mem T), s ≤ t -> t ≤ u -> s ≤ u.
+
+(* Property 6 *)
+
+Axiom set_monotone : forall {T} (s t : Mem T) r v, s ≤ t -> set r v s ≤ set r v t .
+
+(* Property 7 *)
+
+Axiom memle_get : forall {T} (s t : Mem T) r v, s ≤ t -> get r s = Some v -> get r t = Some v.
+
+
+Hint Resolve memle_set memle_get memle_refl set_monotone memle_trans freeFrom_set empty_mem_free : memory.
 End Memory.
 
 
-
-Module Type Empty (Import mem:Memory).
-
-Parameter empty_mem : forall T, Mem T.
-Axiom empty_mem_free : forall T, freeFrom adr0 (empty_mem T).
-
-Hint Resolve empty_mem_free : memory.
-
-End Empty.
-
-Module Type EmptyMem := Memory <+ Empty.
+Lemma rel_eq {T} {R : T -> T -> Prop} x y y' : R x y' -> y = y' -> R x y.
+Proof. intros. subst. auto.
+Qed.
 
 
+(* Additional axioms not used in the paper. *)
+Module Type MAxioms (Import mem: Memory).
+  Axiom set_set : forall T (r : Reg) (v v' : T) (s :  Mem T),
+    set r v (set r v' s) = set r v s.
+  
+  Ltac apply_eq t := eapply rel_eq; [apply t | repeat rewrite set_set; auto].
+End MAxioms.
 
+Module Type SetMem := Memory <+ MAxioms.
 
+(* Extends the memory type with a truncation operation for proper
+modelling of stack frames. *)
 Module Type Truncate (Import mem:Memory).
-
-Parameter truncate : forall {T}, adr -> Mem T -> Mem T.
+Parameter truncate : forall {T}, Reg -> Mem T -> Mem T.
 
 Axiom truncate_monotone : forall {T} (s t : Mem T) r, s ≤ t -> truncate r s ≤ truncate r t.
 Axiom truncate_set : forall {T} (s : Mem T) v r , freeFrom r s -> truncate r (set r v s) = s.
@@ -78,4 +88,4 @@ Hint Resolve truncate_monotone truncate_set : memory.
 
 End Truncate.
 
-Module Type TruncMem := EmptyMem <+ Truncate.
+Module Type TruncMem := SetMem <+ Truncate.
