partial/Tactics.v
@@ -140,20 +140,8 @@ Tactic Notation  (at level 2)    "≤" "{"tactic(t) "}" constr(e) :=
   <|= {{ apply Reach_cle; dist; constructor; solve_memle t }} e .
 
 Tactic Notation  (at level 2)    "=" "{"tactic(t) "}" constr(e) :=
-  match goal with
-  | [|- ?Rel ?lhs ?rhs] => check_rel Reach Rel;
-                           first[ let h := fresh "rewriting" in
-                                  assert(h:rhs = e) by dist' t;
-                                  rewrite h; clear h | fail 2]
-  | _ => fail 1 "goal is not a VM"
-  end.
+   <|= {{ apply Reach_eq;  dist' t}} e.
 
-
-Lemma rel_eq {T} {R : T -> T -> Prop} x y y' : R x y' -> y = y' -> R x y.
-Proof. intros. subst. auto.
-Qed .
-
-Ltac apply_eq t := eapply rel_eq; [apply t | repeat rewrite set_set; auto].
 
 Tactic Notation  (at level 2)    "<==" "{" tactic(t) "}" constr(e) :=
   let tt := try solve[apply trc_step; t; eauto using get_set|apply trc_refl;eauto]
@@ -165,5 +153,4 @@ Tactic Notation  (at level 2)  "begin" constr(rhs) :=
     | [|- ?Rel ?lhs ?rhs'] => check_rel Reach Rel; check_exp rhs rhs'
     | _ => fail 1 "rhs does not match"
   end.
-
 End Calculation.
